add Array.scan{l,r,LM,RM}

Batteries/Data/Array/Basic.lean
@@ -136,10 +136,264 @@ This will perform the update destructively provided that `a` has a reference cou
 abbrev setN (a : Array α) (i : Nat) (x : α) (h : i < a.size := by get_elem_tactic) : Array α :=
   a.set i x
 
+
+
+/--
+  This is guaranteed by the Array docs but it is unprovable.
+  May be asserted to be true in an unsafe context via `Array.unsafe_size_fits_usize
+-/
+abbrev size_fits_usize {a : Array α}: Prop := a.size < USize.size
+
+@[grind .]
+private theorem nat_index_eq_usize_index {n : Nat} {a : Array α} {h : a.size_fits_usize} {hn : n ≤ a.size} :
+    (USize.ofNat n).toNat = n := USize.toNat_ofNat_of_lt' (Nat.lt_of_le_of_lt ‹_› ‹_›)
+
+
+/--
+  This is guaranteed by the Array docs but it is unprovable.
+  Can be used in unsafe functions to write more efficient implementations
+  that avoid boxed integer arithmetic.
+-/
+unsafe def unsafe_size_fits_usize {a: Array α} : Array.size_fits_usize (a := a) := lcProof
+
+
+@[inline]
+private def scanlMFast [Monad m] (f : β → α → m β) (init : β) (as : Array α) (start := 0) (stop := as.size) : m (Array β) :=
+  let stop := min stop as.size
+  let start := min start as.size
+
+  loop f init as
+    (start := USize.ofNat start)
+    (stop := USize.ofNat stop)
+    (h_stop := by grind only [USize.size_eq, USize.ofNat_eq_iff_mod_eq_toNat, = Nat.min_def])
+    (acc := Array.mkEmpty <| stop - start + 1)
+where
+  @[specialize]
+  loop (f : β → α → m β) (init: β) (as: Array α)
+       (start stop : USize)
+       (h_stop : stop.toNat ≤ as.size)
+       (acc : Array β)
+     : m (Array β) := do
+    if h_lt: start < stop then
+      let next ← f init (as.uget start <| Nat.lt_of_lt_of_le h_lt h_stop)
+      loop f next as (start + 1) stop h_stop (acc.push init)
+    else
+      pure <| acc.push init
+  termination_by stop.toNat - min start.toNat stop.toNat
+  decreasing_by
+      have : start < (start + 1) := by grind only [USize.size_eq]
+      grind only [Nat.min_def, USize.lt_iff_toNat_lt]
+
+
+/--
+Fold an effectful function `f` over the array from the left, returning the list of partial results.
+-/
+@[implemented_by scanlMFast]
+def scanlM [Monad m] (f : β → α → m β) (init : β) (as : Array α) (start := 0) (stop := as.size) : m (Array β) :=
+  loop f init as (min start as.size) (min stop as.size) (Nat.min_le_right _ _) #[]
+where
+  loop (f : β → α → m β) (init : β ) (as : Array α)
+       (start stop : Nat)
+       (h_stop : stop ≤ as.size)
+       (acc : Array β)
+     : m (Array β) := do
+    if h_lt : start < stop then
+      loop f (← f init as[start]) as (start + 1) stop h_stop (acc.push init)
+    else
+      pure <| acc.push init
+
+private theorem scanlM_loop_eq_scanlMFast_loop [Monad m]
+    {f : β → α → m β} {init : β} {as : Array α}
+    {h_size : as.size_fits_usize}
+    {start stop : Nat}
+    {h_start : start ≤ as.size}
+    {h_stop : stop ≤ as.size}
+    {acc : Array β}
+  : scanlM.loop f init as start stop h_stop acc
+  = scanlMFast.loop f init as
+      (USize.ofNat start)
+      (USize.ofNat stop)
+      (by rw [USize.toNat_ofNat_of_lt' (Nat.lt_of_le_of_lt h_stop h_size)]; exact h_stop)
+      acc
+  := by
+    generalize h_n : stop - start = n
+    induction n using Nat.strongRecOn generalizing start acc init
+    rename_i n ih
+    rw [scanlM.loop, scanlMFast.loop]
+    have h_stop_usize : (USize.ofNat stop).toNat = stop := nat_index_eq_usize_index (h := h_size) (hn := h_stop)
+    have h_start_usize : (USize.ofNat start).toNat = start := nat_index_eq_usize_index (h := h_size) (hn := h_start)
+    split
+    case isTrue h_lt =>
+      simp_all only [USize.toNat_ofNat', ↓reduceDIte, uget, show USize.ofNat start < USize.ofNat stop by simp_all [USize.lt_iff_toNat_lt]]
+      apply bind_congr
+      intro next
+      have h_start_succ : USize.ofNat start + 1 = USize.ofNat (start + 1) := by
+        simp_all only [← USize.toNat_inj, USize.toNat_add]
+        grind [USize.size_eq]
+      rw [h_start_succ]
+      apply ih (stop - (start + 1)) <;> omega
+    case isFalse h_nlt => grind [USize.lt_iff_toNat_lt]
+
+-- this theorem establishes that given the (unprovable) assumption that as.size < USize.size, the scanlMFast and scanlM are equivalent
+private theorem scanlM_eq_scanlMFast [Monad m]
+    {f : β → α → m β} {init : β} {as : Array α}
+    {h_size : as.size_fits_usize}
+    {start stop : Nat}
+  : scanlM f init as start stop = scanlMFast f init as start stop
+  := by
+    unfold scanlM scanlMFast
+    apply scanlM_loop_eq_scanlMFast_loop
+    simp_all only [gt_iff_lt]
+    apply Nat.min_le_right
+
+
+-- TODO: A lot of grinding here, simplify?
+-- factor out some common helper lemmas?
+-- Note that while scanlMFast and scanlM had almost the exact same structure, scanrMFast and scanrM differ somehat more
+-- The reference implementation works by iterating over `as` backwards, pushing to accumulator, and then reversing it at the end
+-- However, as confirmed via benchmarking, it is faster to initialize the array via `Array.replicate init`, and then iterate backwards
+-- Currently requires a lot of `grinding` to avoid lcProof in the bounds checks.
+@[inline]
+private def scanrMFast [Monad m] (f : α → β → m β) (init : β) (as : Array α) (h_unsafe : as.size_fits_usize) (start := as.size) (stop := 0) : m (Array β) :=
+  let start := min start as.size
+  let stop := min stop start
+
+  loop f init as
+    (start := USize.ofNat start)
+    (stop := USize.ofNat stop)
+    (h_start := by grind only [USize.size_eq, USize.ofNat_eq_iff_mod_eq_toNat, = Nat.min_def])
+    (acc := Array.replicate (start - stop + 1) init)
+    (by grind only [!Array.size_replicate, = Nat.min_def, Array.nat_index_eq_usize_index])
+where
+  @[specialize]
+  loop (f : α → β → m β) (init : β) (as : Array α)
+       (start stop : USize)
+       (h_start : start.toNat ≤ as.size)
+       (acc : Array β)
+       (h_bound : start.toNat - stop.toNat  < acc.size)
+     : m (Array β) := do
+    if h_gt : stop < start then
+      let startM1 := start - 1
+      have : startM1 < start := by grind only [!USize.sub_add_cancel, USize.lt_iff_le_and_ne, USize.lt_add_one, USize.le_zero_iff]
+      have : startM1.toNat < as.size := Nat.lt_of_lt_of_le ‹_› ‹_›
+      have : (startM1 - stop) < (start - stop) := by grind only
+        [!USize.sub_add_cancel, USize.sub_right_inj, USize.add_comm, USize.lt_add_one, USize.add_assoc, USize.add_right_inj]
+
+      let next ← f (as.uget startM1 ‹_›) init
+      loop f next as
+        (start := startM1)
+        (stop := stop)
+        (h_start := Nat.le_of_succ_le_succ (Nat.le_succ_of_le ‹_›))
+        (acc := acc.uset (startM1 - stop) next (by grind only [USize.toNat_sub_of_le, USize.le_of_lt, USize.lt_iff_toNat_lt]))
+        (h_bound := (by grind only [USize.toNat_sub_of_le, = uset_eq_set, = size_set, USize.size_eq]))
+    else
+      pure acc
+  termination_by start.toNat - stop.toNat
+  decreasing_by
+    grind only [USize.lt_iff_toNat_lt, USize.toNat_sub, USize.toNat_sub_of_le, USize.le_iff_toNat_le]
+
+
+@[inline]
+private unsafe def scanrMUnsafe [Monad m] (f : α → β → m β) (init : β) (as : Array α) (start := as.size) (stop := 0) : m (Array β) :=
+  scanrMFast (h_unsafe := Array.unsafe_size_fits_usize) f init as (start := start) (stop := stop)
+
+-- TODO: Prove equivalence of scanlMFast and scanlM as well as scanrMFast (h_unsafe := Array.unsafe_size_fits_usize) and scanrM
+/--
+Folds a monadic function over a list from the left, accumulating the partial results starting with `init`. The
+accumulated value is combined with the each element of the list in order, using `f`.
+
+The optional parameters `start` and `stop` control the region of the array to be folded. Folding
+proceeds from `start` (inclusive) to `stop` (exclusive), so no folding occurs unless `start < stop`.
+By default, the entire array is folded.
+
+Examples:
+```lean example
+example [Monad m] (f : α → β → m α) :
+    Array.scanlM (m := m) f x₀ #[a, b, c] = (do
+      let x₁ ← f x₀ a
+      let x₂ ← f x₁ b
+      let x₃ ← f x₂ c
+      pure #[x₀, x₁, x₂, x₃])
+  := by rfl
+```
+
+```lean example
+example [Monad m] (f : α → β → m α) :
+    Array.scanlM (m := m) f x₀ #[a, b, c] (start := 1) = (do
+      let x₁ ← f x₀ b
+      let x₂ ← f x₁ c
+      pure #[x₀, x₁, x₂])
+  := by rfl
+-/
+@[implemented_by scanrMUnsafe]
+def scanrM [Monad m] (f : α → β → m β) (init : β) (as : Array α) (start := as.size) (stop := 0) : m (Array β) :=
+  let start := min start as.size
+  loop f init as start stop (Nat.min_le_right _ _) #[]
+where
+  loop (f : α → β → m β) (init : β) (as : Array α)
+       (start stop : Nat)
+       (h_start : start ≤ as.size)
+       (acc : Array β)
+     : m (Array β) := do
+    if h_gt : stop < start then
+      let i := start - 1
+      let next ← f as[i] init
+      loop f next as i stop (by omega) (acc.push init)
+    else
+      pure <| acc.push init |>.reverse
+/--
+
+Fold a function `f` over the list from the left, returning the list of partial results.
+```
+scanl (· + ·) 0 #[1, 2, 3] = #[0, 1, 3, 6]
+```
+-/
+@[inline]
+def scanl (f : β → α → β) (init : β) (as : Array α) (start := 0) (stop := as.size) : Array β :=
+  Id.run <| as.scanlM (pure <| f · ·) init start stop
+
+/--
+
+Fold a function `f` over the list from the right, returning the list of partial results.
+```
+scanl (+) 0 #[1, 2, 3] = #[0, 1, 3, 6]
+```
+-/
+@[inline]
+def scanr (f : α → β → β) (init : β) (as : Array α) (start := as.size) (stop := 0) : Array β :=
+  Id.run <| as.scanrM (pure <| f · ·) init start stop
+
 end Array
 
 
 namespace Subarray
+
+/--
+Fold an effectful function `f` over the array from the left, returning the list of partial results.
+-/
+@[inline]
+def scanlM [Monad m] (f : β → α → m β) (init : β) (as : Subarray α) : m (Array β) :=
+  as.array.scanlM f init (start := as.start) (stop := as.stop)
+
+/--
+Fold an effectful function `f` over the array from the right, returning the list of partial results.
+-/
+@[inline]
+def scanrM [Monad m] (f : α → β → m β) (init : β) (as : Subarray α) : m (Array β) :=
+  as.array.scanrM f init (start := as.start) (stop := as.stop)
+
+/--
+Fold a pure function `f` over the array from the left, returning the list of partial results.
+-/
+@[inline]
+def scanl (f : β → α → β) (init : β) (as : Subarray α): Array β :=
+  as.array.scanl f init (start := as.start) (stop := as.stop)
+
+/--
+Fold a pure function `f` over the array from the left, returning the list of partial results.
+-/
+def scanr (f : α → β → β) (init : β) (as : Subarray α): Array β :=
+  as.array.scanr f init (start := as.start) (stop := as.stop)
 
 /--
 Check whether a subarray is empty.
